Minor changes

ref_impl/src/verifier/experiments/fstar_experiments/project/bosqueTerms.fst
@@ -13,7 +13,7 @@ type bosqueTerm =
 | BError : bosqueTerm
 
 (* Definition of getType *)
-val getType_aux : #n:nat 
+val mapBosqueTermType : #n:nat 
   -> (x: sequence bosqueTerm n) 
   -> Tot (sequence bosqueType n) (decreases x)
 val getType : x:bosqueTerm -> Tot bosqueType (decreases x)
@@ -22,12 +22,12 @@ let rec getType x = match x with
 | BInt _ -> BTypeInt
 | BBool _ -> BTypeBool
 | BTuple n SNil -> if (n <> 0) then BTypeError else BTypeEmptyTuple false 
-| BTuple n (SCons y ys) -> BTypeTuple false n (getType_aux #n (SCons y ys))
+| BTuple n (SCons y ys) -> BTypeTuple false n (mapBosqueTermType #n (SCons y ys))
 | BError -> BTypeError
 and 
-getType_aux #n x = match x with
+mapBosqueTermType #n x = match x with
 | SNil -> SNil
-| SCons y ys -> SCons (getType y) (getType_aux ys)
+| SCons y ys -> SCons (getType y) (mapBosqueTermType ys)
 
 (* --------------------------------------------------------------- *)
 (* Casting / Type checkers *)
@@ -46,10 +46,10 @@ let isBool x = match x with
 | BBool _ -> true
 | _ -> false 
 
-val isTuple : n:nat -> (sequence bosqueType n) -> x:bosqueTerm -> Tot bool
-let isTuple n seq x = match x with
-| BTuple m seq' -> n = m 
-  && (eqType (getType (BTuple m seq')) (BTypeTuple false m seq))
+val isTuple : #n:nat -> (sequence bosqueType n) -> x:bosqueTerm -> Tot bool
+let isTuple #n seqTypes x = match x with
+| BTuple m seqTerms -> n = m 
+  && (eqTypeSeq (mapBosqueTermType seqTerms) seqTypes)
 | _ -> false
 
 val isError : bosqueTerm -> Tot bool
